theories/eris/derived_laws.v
@@ -8,30 +8,8 @@ From stdpp Require Import fin_maps.
 From iris.bi Require Import lib.fractional.
 From iris.proofmode Require Import proofmode.
 From clutch.prob_lang Require Import tactics lang notation.
-From clutch.eris Require Export primitive_laws.
+From clutch.eris Require Export primitive_laws array_laws.
 From iris.prelude Require Import options.
-
-(** The [array] connective is a version of [pointsto] that works
-with lists of values. *)
-
-
-Definition array `{!erisGS Σ} (l : loc) (dq : dfrac) (vs : list val) : iProp Σ :=
-  [∗ list] i ↦ v ∈ vs, (l +ₗ i) ↦{dq} v.
-
-(*
-Notation "l ↦∗{ dq } vs" := (array l dq vs)
-  (at level 20, dq custom dfrac at level 1, format "l  ↦∗{ dq } vs") : bi_scope.
-*)
-
-Notation "l ↦∗{ dq } vs" := (array l dq vs)
-  (at level 20, format "l  ↦∗{ dq }  vs") : bi_scope.
-
-Notation "l ↦∗ v" := (l ↦∗{ DfracOwn 1 } v)%I
-                      (at level 20, format "l  ↦∗  v") : bi_scope.
-
-(** We have [FromSep] and [IntoSep] instances to split the fraction (via the
-[AsFractional] instance below), but not for splitting the list, as that would
-lead to overlapping instances. *)
 
 Section lifting.
 
@@ -44,72 +22,6 @@ Section lifting.
   Implicit Types vs : list val.
   Implicit Types sz off : nat.
 
-  (*
-Global Instance array_timeless l q vs : Timeless (array l q vs) := _.
-
-Global Instance array_fractional l vs : Fractional (λ q, l ↦∗{#q} vs)%I := _.
-Global Instance array_as_fractional l q vs :
-  AsFractional (l ↦∗{#q} vs) (λ q, l ↦∗{#q} vs)%I q.
-Proof. split; done || apply _. Qed.
-*)
-
-Lemma array_nil l dq : l ↦∗{dq} [] ⊣⊢ emp.
-Proof. by rewrite /array. Qed.
-
-Lemma array_singleton l dq v : l ↦∗{dq} [v] ⊣⊢ l ↦{dq} v.
-Proof. by rewrite /array /= right_id loc_add_0. Qed.
-
-Lemma array_app l dq vs ws :
-  l ↦∗{dq} (vs ++ ws) ⊣⊢ l ↦∗{dq} vs ∗ (l +ₗ length vs) ↦∗{dq} ws.
-Proof.
-  rewrite /array big_sepL_app.
-  setoid_rewrite Nat2Z.inj_add.
-  by setoid_rewrite loc_add_assoc.
-Qed.
-
-Lemma array_cons l dq v vs : l ↦∗{dq} (v :: vs) ⊣⊢ l ↦{dq} v ∗ (l +ₗ 1) ↦∗{dq} vs.
-Proof.
-  rewrite /array big_sepL_cons loc_add_0.
-  setoid_rewrite loc_add_assoc.
-  setoid_rewrite Nat2Z.inj_succ.
-  by setoid_rewrite Z.add_1_l.
-Qed.
-
-Global Instance array_cons_frame l dq v vs R Q :
-  Frame false R (l ↦{dq} v ∗ (l +ₗ 1) ↦∗{dq} vs) Q →
-  Frame false R (l ↦∗{dq} (v :: vs)) Q | 2.
-Proof. by rewrite /Frame array_cons. Qed.
-
-Lemma update_array l dq vs off v :
-  vs !! off = Some v →
-  ⊢ l ↦∗{dq} vs -∗ ((l +ₗ off) ↦{dq} v ∗ ∀ v', (l +ₗ off) ↦{dq} v' -∗ l ↦∗{dq} <[off:=v']>vs).
-Proof.
-  iIntros (Hlookup) "Hl".
-  rewrite -[X in (l ↦∗{_} X)%I](take_drop_middle _ off v); last done.
-  iDestruct (array_app with "Hl") as "[Hl1 Hl]".
-  iDestruct (array_cons with "Hl") as "[Hl2 Hl3]".
-  assert (off < length vs) as H by (apply lookup_lt_is_Some; by eexists).
-  rewrite length_take min_l; last by lia. iFrame "Hl2".
-  iIntros (w) "Hl2".
-  clear Hlookup. assert (<[off:=w]> vs !! off = Some w) as Hlookup.
-  { apply list_lookup_insert. lia. }
-  rewrite -[in (l ↦∗{_} <[off:=w]> vs)%I](take_drop_middle (<[off:=w]> vs) off w Hlookup).
-  iApply array_app. rewrite take_insert; last by lia. iFrame.
-  iApply array_cons. rewrite length_take min_l; last by lia. iFrame.
-  rewrite drop_insert_gt; last by lia. done.
-Qed.
-
-(** * Rules for allocation *)
-Lemma pointsto_seq_array l dq v n :
-  ([∗ list] i ∈ seq 0 n, (l +ₗ (i : nat)) ↦{dq} v) -∗
-  l ↦∗{dq} replicate n v.
-Proof.
-  rewrite /array. iInduction n as [|n'] "IH" forall (l); simpl.
-  { done. }
-  iIntros "[$ Hl]". rewrite -fmap_S_seq big_sepL_fmap.
-  setoid_rewrite Nat2Z.inj_succ. setoid_rewrite <-Z.add_1_l.
-  setoid_rewrite <-loc_add_assoc. iApply "IH". done.
-Qed.
 
 Lemma wp_allocN E v n s :
   (0 < n)%Z →
