theories/eris/tutorial/basic.v
@@ -1,0 +1,62 @@
+From clutch.eris Require Export eris.
+
+
+Section warmup.
+  Context `{!erisGS Σ}.
+
+  (*
+
+     Eris is a higher-order separation logic to reason about
+     probabilistic programs. The core concept of Eris is
+     "error credits", a novel separation logic resource.
+     Ownership of ε ∈ [0,1] error credits is denoted ↯ ε.
+     When specifying a program e through a triple
+
+     {{{ ↯ ε }}} e @ E {{{ v, RET v; φ v }}}
+
+     the intended meaning of the specification is that the
+     probability of e terminating in a value v that does not
+     satisfy φ v, is at most ε.
+
+     Let's begin with a simple example
+
+  *)
+
+  Definition φ v :iProp Σ:= (⌜v = #true⌝)%I.
+
+  Definition coin_flip_prog : expr :=
+    if: rand #2 <= #0 then #false else #true.
+
+  (*
+
+     Here, rand #2 samples uniformly from the set {0,1,2}.
+     The program therefore returns #false with probability
+     1/3, and #true with probability 2/3. Let's write a
+     specification that captures this idea.
+
+  *)
+
+
+  Lemma coin_flip_spec E :
+    {{{ ↯ (/3) }}} coin_flip_prog @ E {{{ v, RET v; φ v}}}.
+  Proof.
+    (* In Eris, as in Iris, triples are defined in terms
+       of a primitive WP notion.
+    *)
+    iIntros (Ψ) "Herr HΨ".
+    rewrite /coin_flip_prog.
+    wp_apply (wp_rand_err_int _ _ 0 with "[-]").
+    iSplitL "Herr".
+    - simpl.
+      assert (1 + 1 + 1 = 3)%R as -> by lra.
+      iFrame.
+    - iIntros (x) "[[%Hx1  %Hx2] %Hx3]".
+      wp_pures.
+      rewrite bool_decide_eq_false_2; last by lia.
+      wp_pures.
+      iApply "HΨ".
+      done.
+  Qed.
+
+
+End warmup.
