theories/eris/tutorial/hash_interface.v
@@ -1,0 +1,78 @@
+From clutch.eris Require Export eris.
+From stdpp Require Export fin_maps.
+Set Default Proof Using "Type*".
+
+
+(** An interface for hash functions *)
+Class hash_function Σ `{!erisGS Σ} := Hash_Function
+{
+
+  (** * Operations *)
+  init_hash : val;
+
+  (** * Predicates *)
+  hashfun (val_size : nat) (f : val) (m : gmap nat nat): iProp Σ;
+
+  (** * General properties of the predicates
+  #[global] hashkey_timeless γs k v :: Timeless (hashkey γs k v);
+  #[global] conhashfun_persistent γs vs f :: Persistent (hashfun γs vs f);
+  #[global] hashkey_Some_persistent γs k v :: Persistent (hashkey γs k (Some v));
+  *)
+
+
+  hash_init_spec key_size val_size :
+  {{{ True }}}
+    init_hash #key_size #val_size
+  {{{ h, RET h;
+        hashfun val_size h ∅  }}} ;
+
+  hash_query_spec_fresh (k : nat) (avoid : gset nat) (ε εI εO: R) val_size
+    f (m : gmap nat nat) :
+     m !! k = None ->
+     (0 <= εI)%R ->
+     (0 <= εO)%R ->
+     (∀ x, x ∈ avoid → x < S val_size) →
+     (εI * size avoid + εO * (val_size + 1 - size avoid) <= ε * (val_size + 1))%R →
+     {{{ hashfun val_size f m ∗
+           ↯ ε
+     }}}
+       f #k
+       {{{ n, RET #n;
+           ⌜ n < S val_size ⌝%nat ∗
+                   hashfun val_size f (<[k := n]> m) ∗
+        ((⌜n ∉ avoid⌝ ∗ ↯ εO) ∨ (⌜n ∈ avoid⌝ ∗ ↯ εI))
+    }}} ;
+
+  hash_query_spec_prev (k : nat) val_size (v :nat) f (m : gmap nat nat) :
+  m !! k = Some v ->
+  {{{ hashfun val_size f m
+  }}}
+    f #k
+    {{{ RET #v; hashfun val_size f m }}}
+}.
+
+Section derived_lemmas.
+  Context `{!erisGS Σ, !hash_function Σ}.
+
+Lemma wp_insert_basic f val_size m (n : nat)  :
+    m !! n = None →
+    {{{ hashfun val_size f m }}}
+      f #n
+      {{{ (v : nat), RET #v; ⌜ (v < S val_size)%nat ⌝ ∗ hashfun val_size f (<[ n := v ]>m) }}}.
+Proof.
+  iIntros (Hlookup Φ) "Hhash HΦ".
+  iMod (ec_zero) as "Herr".
+  iApply (hash_query_spec_fresh n ∅ 0%R 0%R 0%R val_size with "[$]"); eauto.
+  - lra.
+  - lra.
+  - intro x.
+    rewrite elem_of_empty //.
+  - rewrite size_empty /=.
+    lra.
+  - iModIntro.
+    iIntros (n0) "(%Hsize & Hf & Hset)".
+    iApply ("HΦ" with "[-]").
+    by iFrame.
+Qed.
+
+End derived_lemmas.
